src/Pipit.Context.fst
@@ -1,3 +1,6 @@
+(* Contexts and rows: contexts are lists of types; rows are instances of those
+   types. This module has definitions for binding variables and lemmas about
+   them. *)
 module Pipit.Context
 
 module Map = FStar.FiniteMap.Base
