src/Pipit.Inhabited.fst
@@ -1,3 +1,6 @@
+(* Default or bottom: some interpretations of recursive expressions need an
+   initial value just to seed the computation, even though the value will
+   never be inspected. *)
 module Pipit.Inhabited
 
 class inhabited (a: Type) = {
